bdf2.v
@@ -1,0 +1,90 @@
+Require Import Coq.Arith.Arith.
+Require Import Coq.Bool.Bool.
+Require Export Coq.Strings.String.
+Require Import Coq.Logic.FunctionalExtensionality.
+Require Import Coq.Lists.List.
+Import ListNotations.
+Require Import String.
+Require Import Maps.
+Open Scope string_scope.
+
+Definition ReplicaId := string.
+
+Inductive Replica : Set :=
+| FaultyReplica : Replica
+| NFReplica : Replica.
+
+Definition State := list (Replica * nat).
+
+Definition IsNonFaulty (r:Replica) :  Prop :=
+  match r with 
+    | FaultyReplica => False
+    | NFReplica => True
+  end.
+
+Definition ReplicaFun := State -> string -> State.
+
+Definition NFReplicaFun (st:State) (msg:string):=
+      match st with
+      | nil => [(NFReplica, 0)]
+      | (h, d)::t => (NFReplica, d)::(h, d)::t
+      end
+.
+
+Definition NewReplicaFun (r:Replica) : ReplicaFun :=
+  match r with
+  | FaultyReplica => fun st m => st
+  | NFReplica => NFReplicaFun
+  end.
+
+
+Definition System := list (Replica * ReplicaFun).
+
+Fixpoint ProcessRequest (sys : System) (m : string) (st : State) : State :=
+  match sys with
+  | nil => st
+  | (r,rFun)::t => (rFun (ProcessRequest t m st) m) 
+  end.
+
+Definition dumb1 := [(NFReplica, NewReplicaFun NFReplica); 
+                  (NFReplica, NewReplicaFun NFReplica); (NFReplica, NewReplicaFun NFReplica)].
+Compute ProcessRequest dumb1 "bla" nil.
+
+Fixpoint getLedgerHelper (st:State) (l:nat) : option nat :=
+match st with
+| nil => Some l
+| (NFReplica, l)::t => getLedgerHelper t l
+| (FaultyReplica, _)::t => getLedgerHelper t l
+end.
+
+Fixpoint GetLedger (st:State) : option nat :=
+match st with
+| nil => None
+| (NFReplica, ledger)::t => getLedgerHelper t ledger
+| (FaultyReplica, _)::t => GetLedger t
+end.
+
+Inductive StateValid : State -> Prop :=
+| empty_valid : StateValid nil
+| nonfaulty_valid : forall (r: Replica) (st:State) , IsNonFaulty r -> 
+                StateValid st -> forall d:nat, (GetLedger st) = Some d -> StateValid ((r, d)::st)
+| faulty_valid : forall (r: Replica) (st:State) , ~(IsNonFaulty r) -> StateValid st
+                -> forall d:nat, StateValid ((r, d)::st).
+
+(* Need to link the output d from above to the replica R. We need to know that this came from there, and
+is not just a random d*)
+
+Theorem system_safety : forall (sys : System) (m:string),
+      StateValid (ProcessRequest sys m nil).
+Proof. intros. induction ProcessRequest.
+  - constructor.
+  - destruct a as [r d]. induction r.
+    + apply faulty_valid.
+      { unfold not. intros contra. inversion contra. }
+      { apply IHs. }
+    + apply nonfaulty_valid.
+      { reflexivity. }
+      { apply IHs. }
+      { admit. }
+Admitted.
+
